ops analysis

proof/rejection_sampling/Ops_LeakageAnalysis.ec
@@ -61,6 +61,31 @@ skip. progress. rewrite /copy_f.  rewrite copy_g_comp_1. auto. auto.
 smt().
 qed.
 
+(* DCOPY LEAKAGES  *)
+op dcopy_prefix : leakages_t = LeakFor (0, 64) :: LeakAddr [] ::[].
+op dcopy_step (i : int) : leakages_t = LeakAddr [i] :: LeakAddr [] :: LeakAddr [i] :: [].
+
+op dcopy_g (x : int) : leakages_t.
+axiom dcopy_g_comp_1 x : x <= 0 => dcopy_g x = [].
+axiom dcopy_g_comp_2 x : 0 <  x => dcopy_g x = dcopy_step (x-1) ++ dcopy_g (x - 1).
+
+op dcopy_f (x : int) : leakages_t = dcopy_g x ++ dcopy_prefix.
+
+lemma dbn_copy_leakages start_l :
+   hoare [ M(Syscall).dbn_copy : M.leakages = start_l 
+     ==> M.leakages = dcopy_f 64 ++ start_l ].
+proof. 
+proc.
+sp.  elim*. progress.
+conseq (_: M.leakages = dcopy_prefix ++ start_l /\ i = 0 /\ aux = 64 ==> _).
+progress.
+while (aux = 64 /\ 0 <= i /\ i <= 64 /\ M.leakages = dcopy_f i ++ start_l).
+wp.  skip.  progress. 
+simplify. smt(). smt(). rewrite /dcopy_f. rewrite (dcopy_g_comp_2 (i{hr} +1)).  smt(). simplify. rewrite /dcopy_step. simplify. auto.
+skip. progress. rewrite /dcopy_f.  rewrite dcopy_g_comp_1. auto. auto. 
+smt().
+qed.
+
 
 
 (* set0 LEAKAGES  *)
@@ -170,11 +195,338 @@ smt().
 qed.
 
 
-(* mulm LEAKAGES  *)
-op mulm_t :  leakages_t.
 
-lemma mulm_leakages start_l :
-   hoare [ M(Syscall).mulm : M.leakages = start_l 
-                ==> M.leakages = mulm_t ++ start_l ].
+(* mul1 LEAKAGES  *)
+op mul1_prefix : leakages_t = LeakFor (1, 32) :: LeakAddr [] :: LeakAddr [0] :: LeakAddr [] :: LeakAddr [1] :: 
+LeakAddr [] :: LeakAddr [] :: LeakAddr [0] :: LeakAddr [] :: LeakAddr [] :: [].
+op mul1_step (x : int) : leakages_t = LeakAddr [x] :: LeakAddr [] :: LeakAddr [] :: LeakAddr [] :: LeakAddr
+                                                                   [x] :: 
+LeakAddr [] :: LeakAddr [x + 1] :: LeakAddr [] :: LeakAddr [] :: 
+LeakAddr [x] :: LeakAddr [] :: [].
+
+op mul1_suffix : leakages_t = LeakAddr [32] :: LeakAddr [] :: LeakAddr [] :: LeakAddr [32] :: [].
+
+op mul1_g (x : int) : leakages_t.
+axiom mul1_g_comp_1 x : x = 1 => mul1_g x = [].
+axiom mul1_g_comp_2 x : 1 <  x => mul1_g x = mul1_step (x-1) ++ mul1_g (x - 1).
+
+op mul1_f (x : int) : leakages_t = mul1_suffix ++ mul1_g x ++ mul1_prefix.
+
+lemma mul1_leakages start_l :
+   hoare [ M(Syscall).mul1 : M.leakages = start_l 
+     ==> M.leakages = mul1_f 32 ++ start_l ].
+proof. 
+proc.
+sp.  elim*. progress.
+conseq (_: M.leakages = mul1_prefix ++ start_l /\ i = 1 ==> _).
+progress. wp.
+while (1 <= i /\ i <= 32 /\ M.leakages = mul1_g i ++ mul1_prefix ++ start_l).
+wp.  skip.  progress. 
+smt(). smt(). 
+rewrite /mul1_f. rewrite (mul1_g_comp_2 (i{hr} +1)).  smt(). simplify. rewrite /mul1_step. simplify. auto.
+skip. progress. rewrite /mul1_f.  rewrite mul1_g_comp_1. auto. auto. 
+smt().
+qed.
+
+
+(* mul1acc LEAKAGES  *)
+op mul1acc_prefix  : leakages_t = LeakFor (0, 31) :: LeakAddr [] :: LeakAddr [] :: [].
+
+op mul1acc_suffix (kkk : int) : leakages_t =  LeakAddr [32 +  kkk] :: LeakAddr [] :: LeakAddr [] :: LeakAddr
+                                                               [32 +
+                                                                 kkk] :: 
+LeakAddr [32 +  kkk] :: LeakAddr [] :: LeakAddr [] :: LeakAddr
+                                                               [32 +
+                                                                 kkk] :: 
+LeakAddr [31 +  kkk] :: LeakAddr [] :: LeakAddr [] :: LeakAddr
+                                                               [31 +
+                                                                 kkk] :: 
+LeakAddr [] :: LeakAddr [32 +  kkk] :: LeakAddr [] :: LeakAddr [] :: 
+LeakAddr [31] :: LeakAddr [] :: [].
+
+op mul1acc_step (kk i : int) : leakages_t = LeakAddr [kk + i + 1] :: LeakAddr [] :: LeakAddr [] :: LeakAddr
+                                                                 [kk +
+                                                                  i + 1] :: 
+LeakAddr [kk + i] :: LeakAddr [] :: LeakAddr [] :: LeakAddr
+                                                             [kk + i] :: 
+LeakAddr [] :: LeakAddr [] :: LeakAddr [] :: LeakAddr [i] :: LeakAddr [] :: [].
+
+
+op mul1acc_g (kk x : int) : leakages_t.
+axiom mul1acc_g_comp_1 kk x : x = 0 => mul1acc_g kk x = [].
+axiom mul1acc_g_comp_2 kk x : 0 < x => mul1acc_g kk x = mul1acc_step kk (x-1) ++ mul1acc_g kk (x - 1).
+
+op mul1acc_f (kk x : int) : leakages_t = mul1acc_suffix kk ++ mul1acc_g kk x ++ mul1acc_prefix.
+
+lemma mul1acc_leakages start_l kkk :
+   hoare [ M(Syscall).mul1acc : M.leakages = start_l  /\ k = kkk
+     ==> M.leakages = mul1acc_f (to_uint kkk) 31 ++ start_l ].
+proof. 
+proc.
+sp.  elim*. progress.
+conseq (_: M.leakages = mul1acc_prefix ++ start_l /\ i = 0 /\ aux = 31 /\ (to_uint kkk) = kk ==> _).
+progress. wp.
+while (aux = 31 /\ 0 <= i /\ i <= 31 /\ M.leakages = mul1acc_g kk i ++ mul1acc_prefix ++ start_l /\ kk = (to_uint kkk)).
+wp.  skip.  progress. 
+smt(). smt(). 
+rewrite (mul1acc_g_comp_2 (to_uint kkk) (i{hr}+1)).  smt(). simplify. rewrite /mul1acc_step. simplify. auto.
+skip. progress. rewrite mul1acc_g_comp_1. auto. auto. 
+simplify.
+have -> : i0 = 31. smt().
+rewrite /mul1acc_f. 
+rewrite /mul1acc_suffix. simplify. auto.
+qed.
+
+(* bn_muln LEAKAGES  *)
+op bn_muln_prefix : leakages_t = LeakFor (1, 32) :: LeakAddr [] :: (mul1_f 32 ++ [LeakAddr []; LeakAddr [0]]).
+op bn_muln_step (i : int) : leakages_t = mul1acc_f (to_uint ((of_int i))%W64) 31 ++
+ [LeakAddr [] ; LeakAddr [] ; LeakAddr [i]] .
+
+op bn_muln_g (x : int) : leakages_t.
+axiom bn_muln_g_comp_1 x : x = 1 => bn_muln_g x = [].
+axiom bn_muln_g_comp_2 x : 1 <  x => bn_muln_g x = bn_muln_step (x-1) ++ bn_muln_g (x - 1).
+
+op bn_muln_f (x : int) : leakages_t = bn_muln_g x ++ bn_muln_prefix.
+
+lemma bn_muln_leakages start_l :
+   hoare [ M(Syscall).bn_muln : M.leakages = start_l 
+     ==> M.leakages = bn_muln_f 32 ++ start_l ].
+proof. 
+proc.
+seq 12 : (i = 1 /\ M.leakages = [LeakFor (1, 32) ; LeakAddr [] ] ++ mul1_f 32 ++ [LeakAddr []; LeakAddr [0]] ++ start_l).
+wp. sp. elim*. progress.
+call (mul1_leakages ([LeakAddr [] ; LeakAddr [0] ] ++ start_l)).
+skip. progress. smt(@List).
+
+while (1 <= i /\ i <= 32 /\ M.leakages = bn_muln_g i ++ bn_muln_prefix ++ start_l).
+wp.  
+sp. elim*. progress.
+
+exists* i. elim*. move => i_var.
+call (mul1acc_leakages ([LeakAddr [] ; LeakAddr [] ; LeakAddr [i_var]] ++ leakages) (W64.of_int i_var)).
+skip. progress.
+smt().
+smt().
+rewrite (bn_muln_g_comp_2 (i{hr}+1)). smt(). simplify. rewrite /bn_muln_step.
+pose xxx := mul1acc_f (to_uint ((of_int i{hr}))%W64) 31.
+do ? rewrite - catA.
+congr.
+congr. congr. 
+smt(@List).
+skip.
+progress.
+rewrite bn_muln_g_comp_1. auto. simplify.
+rewrite /bn_muln_prefix. auto.
+smt().
+qed.
+
+
+(* div2 LEAKAGES  *)
+op div2_prefix (k : int) : leakages_t = LeakFor (0, k) :: LeakAddr [] :: [].
+op div2_step (i : int) : leakages_t = LeakAddr [i] :: LeakAddr [64 + i] :: [].
+
+op div2_g (x : int) : leakages_t.
+axiom div2_g_comp_1 x : x = 0 => div2_g x = [].
+axiom div2_g_comp_2 x : 0 <  x => div2_g x = div2_step (x-1) ++ div2_g (x - 1).
+
+op div2_f (x k : int) : leakages_t = div2_g x ++ div2_prefix k.
+
+lemma div2_leakages start_l kk :
+   hoare [ M(Syscall).div2 : M.leakages = start_l  /\ kk = k /\ 0 <= k
+     ==> M.leakages = div2_f kk kk ++ start_l ].
+proof. 
+proc.
+sp.  elim*. progress.
+conseq (_: 0 <= k /\ aux = k /\ M.leakages = div2_prefix k ++ start_l /\ i = 0 /\ k = kk ==> _).
+progress.
+while (aux = k /\ 0 <= i /\ i <= k /\ M.leakages = div2_f i k ++ start_l /\ k = kk).
+wp.  skip.  progress. 
+smt(). smt(). 
+rewrite /div2_f. rewrite (div2_g_comp_2 (i{hr}+1)).  smt(). simplify. rewrite /div2_step. simplify. auto.
+skip. progress.  rewrite /div2_f. rewrite div2_g_comp_1. auto. auto. 
+have -> : i0 = k{hr}. smt(). auto.
+qed.
+
+
+
+(* bn_shrink LEAKAGES  *)
+op bn_shrink_prefix : leakages_t = LeakFor (0, 32) :: LeakAddr [] :: [].
+op bn_shrink_step (i : int) : leakages_t = LeakAddr [i] :: LeakAddr [i] :: [].
+
+op bn_shrink_g (x : int) : leakages_t.
+axiom bn_shrink_g_comp_1 x : x = 0 => bn_shrink_g x = [].
+axiom bn_shrink_g_comp_2 x : 0 <  x => bn_shrink_g x = bn_shrink_step (x-1) ++ bn_shrink_g (x - 1).
+
+op bn_shrink_f (x : int) : leakages_t = bn_shrink_g x ++ bn_shrink_prefix.
+
+lemma bn_shrink_leakages start_l :
+   hoare [ M(Syscall).bn_shrink : M.leakages = start_l 
+     ==> M.leakages = bn_shrink_f 32 ++ start_l ].
+proof. 
+proc.
+sp.  elim*. progress.
+conseq (_: M.leakages = bn_shrink_prefix ++ start_l /\ i = 0 ==> _).
+progress.
+while (0 <= i /\ i <= 32 /\ M.leakages = bn_shrink_f i ++ start_l).
+wp.  skip.  progress. 
+smt(). smt(). 
+rewrite /bn_shrink_f. rewrite (bn_shrink_g_comp_2 (i{hr} +1)).  smt(). simplify. rewrite /bn_shrink_step. simplify. auto.
+skip. progress. rewrite /bn_shrink_f.  rewrite bn_shrink_g_comp_1. auto. auto. 
+smt().
+qed.
+
+
+
+(* SUBTRACTION LEAKAGES  *)
+op dsub_prefix : leakages_t = 
+  [LeakFor (1, 64); LeakAddr []; LeakAddr [0]; LeakAddr []; 
+    LeakAddr []; LeakAddr [0]; LeakAddr [0]].
+
+op dsub_step (i : int) : leakages_t = 
+  [LeakAddr [i] ; LeakAddr [] ; LeakAddr [] ; LeakAddr [i] ; 
+    LeakAddr [i] ].
+
+
+op dsub_g (x : int) : leakages_t.
+axiom dsub_g_comp_1 x : x <= 1 => dsub_g x = [].
+axiom dsub_g_comp_2 x : 1 <  x => dsub_g x = dsub_step (x-1) ++ dsub_g (x - 1).
+
+op dsub_f (x : int) : leakages_t = dsub_g x ++ dsub_prefix.
+
+
+lemma dbn_subc_leakages start_l :
+  hoare [ M(Syscall).dbn_subc : M.leakages = start_l 
+            ==> M.leakages = dsub_f 64 ++ start_l ].
+proof. 
+proc.
+sp.  elim*. progress.
+conseq (_: M.leakages = dsub_prefix ++ start_l /\ i = 1 /\ aux_1 = 64 ==> _).
+progress.
+while (aux_1 = 64 /\ 0 < i /\ i <= 64 /\ M.leakages = dsub_f i ++ start_l).
+wp.  skip.  progress. 
+simplify. smt(). smt(). rewrite /dsub_f. rewrite (dsub_g_comp_2 (i{hr} +1)).  smt(). simplify. rewrite /dsub_step. simplify. auto.
+skip. progress. rewrite /dsub_f.  rewrite dsub_g_comp_1. auto. auto.
+smt().
+qed.
+
+
+
+(* bn_expand LEAKAGES  *)
+op bn_expand_prefix : leakages_t = LeakFor (0, 32) :: LeakAddr [] :: [].
+op bn_expand_step (i : int) : leakages_t = LeakAddr [i] :: LeakAddr [i] :: [].
+op bn_expand_step2 (i : int) : leakages_t = LeakAddr [i] :: LeakAddr [] :: [].
+
+op bn_expand_g (x : int) : leakages_t.
+axiom bn_expand_g_comp_1 x : x = 0 => bn_expand_g x = [].
+axiom bn_expand_g_comp_2 x : 0 <  x => bn_expand_g x = bn_expand_step (x-1) ++ bn_expand_g (x - 1).
+
+op bn_expand_h (x : int) : leakages_t.
+axiom bn_expand_h_comp_1 x : x = 32 => bn_expand_h x = [].
+axiom bn_expand_h_comp_2 x : 32 < x => bn_expand_h x = bn_expand_step2 (x-1) ++ bn_expand_h (x - 1).
+
+
+op bn_expand_f (x : int) : leakages_t = bn_expand_h (2 * x) ++ [LeakFor (32, 64) ; LeakAddr [] ] ++ bn_expand_g x ++ bn_expand_prefix.
+
+lemma bn_expand_leakages start_l :
+   hoare [ M(Syscall).bn_expand : M.leakages = start_l 
+     ==> M.leakages = bn_expand_f 32 ++ start_l ].
+proof. 
+proc.
+seq 4 : (M.leakages =  bn_expand_g 32 ++ bn_expand_prefix ++ start_l).
+sp.  elim*. progress.
+conseq (_: M.leakages = bn_expand_prefix ++ start_l /\ i = 0 ==> _).
+progress.
+while (0 <= i /\ i <= 32 /\ M.leakages = bn_expand_g i ++ bn_expand_prefix ++ start_l).
+wp.  skip.  progress. 
+smt(). smt(). 
+rewrite (bn_expand_g_comp_2 (i{hr} +1)).  smt(). simplify. rewrite /bn_expand_step. simplify. auto.
+skip. progress.  rewrite bn_expand_g_comp_1. auto. auto. 
+smt().
+sp. elim*. progress.
+rewrite /bn_expand_f. simplify.
+conseq (_: i = 32 /\ aux = 64 /\ M.leakages = LeakFor (32, 64) :: LeakAddr [] :: bn_expand_g 32 ++ bn_expand_prefix ++ start_l ==> _).
+progress.
+while (aux = 64 /\ 32 <= i /\ i <= 64 
+  /\ M.leakages = (bn_expand_h i ++ LeakFor (32, 64) :: LeakAddr [] :: 
+                   bn_expand_g 32 ++ bn_expand_prefix ++ start_l)).
+wp.  skip.  progress. 
+smt(). smt(). 
+rewrite (bn_expand_h_comp_2 (i{hr} +1)).  smt(). simplify.
+ rewrite /bn_expand_step2. simplify. auto.
+skip. progress. simplify.
+rewrite bn_expand_h_comp_1. auto. 
+simplify. auto. smt(@List).
+qed.
+
+
+(* dbn_cmov LEAKAGES  *)
+op dbn_cmov_prefix : leakages_t = LeakFor (0, 64) :: LeakAddr [] :: [].
+op dbn_cmov_step (i : int) : leakages_t = LeakAddr [i] :: LeakAddr [] :: LeakAddr [] :: LeakAddr [i] :: 
+LeakAddr [i] :: [].
+
+op dbn_cmov_g (x : int) : leakages_t.
+axiom dbn_cmov_g_comp_1 x : x = 0 => dbn_cmov_g x = [].
+axiom dbn_cmov_g_comp_2 x : 0 <  x => dbn_cmov_g x = dbn_cmov_step (x-1) ++ dbn_cmov_g (x - 1).
+
+op dbn_cmov_f (x : int) : leakages_t = dbn_cmov_g x ++ dbn_cmov_prefix.
+
+lemma dbn_cmov_leakages start_l :
+   hoare [ M(Syscall).dbn_cmov : M.leakages = start_l 
+     ==> M.leakages = dbn_cmov_f 64 ++ start_l ].
+proof. 
+proc.
+sp.  elim*. progress.
+conseq (_: M.leakages = dbn_cmov_prefix ++ start_l /\ i = 0 /\ aux = 64 ==> _).
+progress.
+while (0 <= i /\ i <= 64 /\ aux = 64 /\ M.leakages = dbn_cmov_f i ++ start_l).
+wp.  skip.  progress. 
+smt(). smt(). 
+rewrite /dbn_cmov_f. rewrite (dbn_cmov_g_comp_2 (i{hr} +1)).  smt(). simplify. rewrite /dbn_cmov_step.
+progress. skip. progress.  rewrite /dbn_cmov_f. rewrite dbn_cmov_g_comp_1. auto. auto. 
+smt().
+qed.
+
+(* dcminusP LEAKAGES  *)
+op dcminusP_f  : leakages_t = 
+ dbn_cmov_f 64 ++ [LeakAddr []] ++ dsub_g 64 ++ dsub_prefix ++ [LeakAddr []] ++
+dcopy_g 64 ++ dcopy_prefix ++ [LeakAddr []] .
+
+lemma dcminusP_leakages start_l :
+   hoare [ M(Syscall).dcminusP : M.leakages = start_l 
+     ==> M.leakages = dcminusP_f  ++ start_l ].
+proof. 
+proc.
+pose suf1 :=  [LeakAddr []] ++ start_l.
+seq 4 : (M.leakages = dcopy_f 64 ++ suf1 ).
+wp.  call (dbn_copy_leakages suf1). simplify. wp. skip. progress. auto.
+
+pose suf2 :=  [LeakAddr []] ++ dcopy_f 64 ++ suf1.
+seq 3 : (M.leakages = dsub_f 64 ++ suf2).
+wp.  call (dbn_subc_leakages suf2). wp. skip. progress.
+
+pose suf3 :=  [LeakAddr []] ++ dsub_f 64 ++ suf2.
+seq 3 : (M.leakages = dbn_cmov_f 64 ++ suf3).
+wp.  call (dbn_cmov_leakages suf3). wp. skip. progress.
+skip.
+progress. rewrite /suf3 /suf2 /suf1.
+do ? rewrite catA. rewrite /dcminusP_f.
+auto.
+qed.
+
+(* bn_breduce LEAKAGES  *)
+op bn_breduce_f (x : int) : leakages_t.
+
+lemma bn_breduce_leakages start_l :
+   hoare [ M(Syscall).bn_breduce : M.leakages = start_l 
+     ==> M.leakages = bn_breduce_f 32 ++ start_l ].
+proof. 
+proc. 
 admitted.
 
+(* mulm LEAKAGES  *)
+op mulm_t : leakages_t.
+lemma mulm_leakages start_l : 
+   hoare [ M(Syscall).mulm : M.leakages = start_l 
+                ==> M.leakages = mulm_t ++ start_l ].
+proof. 
+admitted.
